transl_step done
The previous problem was "extends", which doesn't hold here:
After alloc and free, the memory state changes.

Particulary, nextblock will be different after alloc and free,
since alloc increases it and free doesn't change it.  This violates
extends, which requires the same nextblock value (see mext_next).

Now we use injection and it seems good.

Seccompproof.v
@@ -60,6 +60,51 @@ Proof.
   exact (Genv.find_var_info_transf_partial transl_fundef _ TRANSL).
 Qed.
 
+Definition mem_inj := Mem.mem_inj inject_id.
+
+Lemma inj_refl:
+  forall m, mem_inj m m.
+Proof.
+  intros.
+  constructor; intros; unfold inject_id in H; inv H.
+
+  replace (ofs + 0) with ofs by omega.
+  auto.
+
+  apply Z.divide_0_r.
+
+  replace (ofs + 0) with ofs by omega.
+  apply memval_lessdef_refl.
+Qed.
+
+Lemma inj_trans:
+  forall m1 m2 m3,
+  mem_inj m1 m2 -> mem_inj m2 m3 -> mem_inj m1 m3.
+Proof.
+  unfold mem_inj.
+  apply Mem.mem_inj_compose.
+Qed.
+
+Lemma free_alloc_inj:
+  forall m1 m2 b lo hi m2',
+  Mem.alloc m1 lo hi = (m2, b) ->
+  Mem.free m2 b lo hi = Some m2' ->
+  mem_inj m1 m2'.
+Proof.
+  intros.
+  apply (Mem.free_right_inj inject_id m1 m2 b lo hi m2').
+  apply (Mem.alloc_right_inj inject_id m1 m1 lo hi b m2).
+  exact (inj_refl m1). auto. auto.
+
+  intros.
+  apply (Mem.fresh_block_alloc m1 lo hi m2 b).
+  auto.
+  apply (Mem.perm_valid_block m1 b') in H2.
+  unfold inject_id in H1.
+  inv H1.
+  auto.
+Qed.
+
 Inductive match_states: Seccomp.state -> Cminor.state -> Prop :=
   | match_state:
       forall a x sm f c m tf ts tk tsp te tm b tm'
@@ -71,13 +116,13 @@ Inductive match_states: Seccomp.state -> Cminor.state -> Prop :=
         (MSP: tsp = Vptr b Int.zero)
 (*        (MPERM: Mem.range_perm tm b 0 tf.(fn_stackspace) Cur Freeable) *)
         (MFREE: Mem.free tm b 0 tf.(fn_stackspace) = Some tm')
-        (MEXT: Mem.extends m tm'),
+        (MINJ: mem_inj m tm'),
       match_states (Seccomp.State a x sm f c m)
                    (Cminor.State tf ts tk tsp te tm)
   | match_callstate:
       forall fd m tfd targs tk tm
         (TF: transl_fundef fd = OK tfd)
-        (MEXT: Mem.extends m tm)
+        (MINJ: mem_inj m tm)
         (MARGS: targs = nil)
         (MK: call_cont tk = Kstop),
       match_states (Seccomp.Callstate fd m)
@@ -85,7 +130,7 @@ Inductive match_states: Seccomp.state -> Cminor.state -> Prop :=
   | match_returnstate:
       forall v m tv tk tm
         (MV: Vint v = tv)
-        (MEXT: Mem.extends m tm)
+        (MINJ: mem_inj m tm)
         (MK: tk = Kstop),
       match_states (Seccomp.Returnstate v m)
                    (Cminor.Returnstate tv tk tm)
@@ -114,7 +159,7 @@ Proof.
 
   (* match states S R *)
   constructor; auto.
-  apply Mem.extends_refl.
+  apply inj_refl.
 Qed.
 
 Lemma transl_final_states:
@@ -253,5 +298,13 @@ Proof.
   econstructor; auto.
   unfold transl_function; unfold transl_funbody; rewrite EQ; auto.
   exact e.
+
+  apply (free_alloc_inj tm
+    (fst (Mem.alloc tm 0 (seccomp_memwords * 4)))
+    (snd (Mem.alloc tm 0 (seccomp_memwords * 4)))
+    0 (seccomp_memwords * 4) _) in e.
+  apply (inj_trans m tm _); auto.
+  auto.
+Qed.
 
 (* End PRESERVATION. *)
